= Rationalizing the denominator

In general, you want to avoid radicals in the denominator. To rationalize the denominator, multiply both the numerator and the denominator by the conjugate of the denominator.

$
  &1 / (1 + sqrt(2))\
  &= 1 / (1 + sqrt(2)) dot (1 - sqrt(2)) / (1 - sqrt(2)) \
  &= (1 - sqrt(2)) / ((1 + sqrt(2))(1- sqrt(2))) \
  &= (1 - sqrt(2)) / (1^2 - sqrt(2)^2) \
  &= (1 - sqrt(2)) / (1 - 2) \
  &= (1 - sqrt(2)) / (-1) \
  &= -1 + sqrt(2)
$

== Exercises

1.

$
  &(1 + sqrt(8)) / (sqrt(9) - sqrt(2))\
  &= ((1+sqrt(8))(sqrt(9)+sqrt(2))) / 7\
  &= (sqrt(9) + 3sqrt(8) + sqrt(2) + sqrt(16))/ 7\
  &= (3 + 6sqrt(2) + sqrt(2) + 4)/7\
  &= (7 + 7sqrt(2))/7\
  &= 1 + sqrt(2)
$
